examples/pick_left.v
@@ -1,0 +1,99 @@
+(* Add LoadPath "C:\Users\Ziga\Documents\Ziga_podatki\repositories\eeff-formalization\syntax". *)
+(* Add LoadPath "C:\Users\Ziga\Documents\Ziga_podatki\repositories\eeff-formalization\type_system". *)
+(* Add LoadPath "C:\Users\Ziga\Documents\Ziga_podatki\repositories\eeff-formalization\substitution". *)
+(* Add LoadPath "C:\Users\Ziga\Documents\Ziga_podatki\repositories\eeff-formalization\operational_semantics". *)
+(* Add LoadPath "C:\Users\Ziga\Documents\Ziga_podatki\repositories\eeff-formalization\logic". *)
+Add LoadPath "E:\Ziga_Podatki\faks\eeff-formalization\syntax".
+Add LoadPath "E:\Ziga_Podatki\faks\eeff-formalization\type_system".
+Add LoadPath "E:\Ziga_Podatki\faks\eeff-formalization\substitution".
+Add LoadPath "E:\Ziga_Podatki\faks\eeff-formalization\operational_semantics".
+Add LoadPath "E:\Ziga_Podatki\faks\eeff-formalization\logic".
+
+Require Export syntax_lemmas substitution_lemmas type_lemmas logic_lemmas String.
+Open Scope string_scope.
+
+Example sig := (SigU (SigØ) ("choose") TyUnit (TyΣ TyUnit TyUnit)).
+
+Lemma sig_wf:
+  wf_sig sig.
+Proof.
+unfold sig. apply WfSigU.
+- apply WfSigØ.
+- simpl. auto.
+- apply WfTyUnit.
+- apply WfTyΣ; apply WfTyUnit.
+Qed.
+
+Example eq_idem := (EqsU (EqsØ) CtxØ (TCtxU TCtxØ TyUnit)
+  (TApp ("z", 0) Unit)
+  (TOp "choose" Unit "y" 
+    (TΣMatch (Var ("y", 0)) 
+      "_" (TApp ("z", 0) Unit)
+      "_" (TApp ("z", 0) Unit)))
+).
+
+Lemma eq_idem_wf:
+  wf_eqs eq_idem sig.
+Proof.
+assert (wf_ctx CtxØ) by apply WfCtxØ.
+assert (wf_vtype TyUnit) by apply WfTyUnit.
+assert (forall Γ, wf_ctx Γ -> has_vtype Γ Unit TyUnit).
+{ intros Γ wf. apply TypeV. auto. apply WfTyUnit. apply TypeUnit. }
+unfold eq_idem. apply WfEqsU; auto.
+- apply WfEqsØ.
+- apply WfTCtxU. apply WfTCtxØ. apply WfTyUnit.
+- apply sig_wf.
+- eapply WfTApp; eauto.
+- eapply WfTOp.
+  + unfold sig. simpl. reflexivity.
+  + auto.
+  + eapply WfTΣMatch.
+    * apply TypeV. apply WfCtxU. auto. apply WfTyΣ; auto.
+      apply WfTyΣ; eauto. apply TypeVar. simpl. auto.
+    * eapply WfTApp. apply H1.
+      apply WfCtxU. apply WfCtxU. auto. apply WfTyΣ. all: auto.
+    * eapply WfTApp. apply H1.
+      apply WfCtxU. apply WfCtxU. auto. apply WfTyΣ. all: auto.
+Qed.
+
+Example handler :=
+  Handler "x" (Ret (Var ("x", 0)))
+  (CasesU CasesØ
+    "choose" "k" "x" (App (Var ("k", 1)) (Inl Unit))).
+
+Lemma handler_types:
+  has_vtype CtxØ handler (TyHandler (CTy TyInt sig eq_idem) (CTy TyInt SigØ EqsØ))
+.
+assert (wf_ctype (CTy TyInt sig eq_idem)).
+{ apply WfCTy. apply WfTyInt. apply sig_wf. apply eq_idem_wf. }
+assert (wf_ctype (CTy TyInt SigØ EqsØ)).
+{ apply WfCTy. apply WfTyInt. apply WfSigØ. apply WfEqsØ. }
+apply TypeV. apply WfCtxØ. apply WfTyHandler; auto.
+apply TypeHandler.
++ assert (wf_ctx (CtxU CtxØ TyInt)).
+  apply WfCtxU. apply WfCtxØ. apply WfTyInt. 
+  apply TypeC; auto.
+  apply TypeRet. apply TypeV. auto. apply WfTyInt.
+  apply TypeVar. simpl. auto.
++ assert (wf_ctx CtxØ) by apply WfCtxØ.
+  apply TypeH; auto. apply sig_wf.
+  apply TypeCasesU. 
+  - simpl. auto.
+  - apply TypeH; auto. apply WfSigØ.
+    apply TypeCasesØ.
+  - assert (wf_ctx (CtxU (CtxU CtxØ (TyFun (TyΣ TyUnit TyUnit) (CTy TyInt SigØ EqsØ))) TyUnit)).
+    { assert (wf_vtype TyUnit) by apply WfTyUnit.
+      apply WfCtxU. apply WfCtxU. auto. apply WfTyFun. apply WfTyΣ. all: auto. }
+    apply TypeC; auto.
+    eapply TypeApp.
+    * apply TypeV; auto. inv H2. inv H5. eauto.
+      apply TypeVar. simpl. auto.
+    * apply TypeV; auto. apply WfTyΣ; apply WfTyUnit.
+      apply TypeInl. apply TypeV; auto. apply WfTyUnit.
+      apply TypeUnit.
++ apply Respects.
+  apply WfCtxØ. apply sig_wf. auto. apply eq_idem_wf.
+  apply RespectEqsU.
+  apply Respects. apply WfCtxØ. apply sig_wf. auto. apply WfEqsØ.
+  apply RespectEqsØ.
+  simpl. unfold c_subs2_out. unfold c_subs_out. unfold c_subs. simpl.
